Simplify the benchmark a bit

benchmarks/binomial_heap/shared/AdjustedBinomialHeap.v
@@ -1,145 +1,137 @@
-(** First-order adaptation of:
+(** Original source copied from:
     https://github.com/CertiCoq/certicoq/blob/59f110359ed57550a746124441f20b993774af78/tests/lib/Binom.v
 
-    License terms: [../NOTICE]. *)
+    License terms: [../NOTICE].
 
-From Stdlib Require Import Arith List.
+    The adapted and reified implementation is in
+    [rocq/binomial_heap/BinomialHeap.v]. *)
+
+Require Import Coq.Arith.Arith List.
 From coqutil Require Import dlet.
 
 Import ListNotations.
-Import Nat.
-Open Scope nat_scope.
-
-Notation "'let/d' x := val 'in' body" :=
-  (dlet val (fun x => body))
-  (at level 200, x name, body at level 200).
-
+Import Nat. (* For 8.5.0 *)
 Definition key := nat.
 
 Inductive tree : Type :=
-| Node : key -> tree -> tree -> tree
-| Leaf : tree.
+|  Node: key -> tree -> tree -> tree
+|  Leaf : tree.
 
 Definition priqueue := list tree.
 
 Definition empty : priqueue := nil.
 
-Notation "a >? b" := (Nat.ltb b a)
-  (at level 70, only parsing) : nat_scope.
+Notation  "a >? b" := (ltb b a) (at level 70, only parsing) : nat_scope.
 
-Definition smash (t u : tree) : tree :=
-  match t, u with
-  | Node x t1 Leaf, Node y u1 Leaf =>
-      if x >? y then Node x (Node y u1 t1) Leaf
-      else Node y (Node x t1 u1) Leaf
-  | _, _ => Leaf
+Definition smash (t u:  tree) : tree :=
+  match t , u with
+  |  Node x t1 Leaf, Node y u1 Leaf =>
+                   if  x >? y then Node x (Node y u1 t1) Leaf
+                                else Node y (Node x t1 u1) Leaf
+  | _ , _ => Leaf  (* arbitrary bogus tree *)
   end.
 
-Fixpoint carry (q : list tree) (t : tree) : list tree :=
+Fixpoint carry (q: list tree) (t: tree) : list tree :=
   match q, t with
-  | nil, Leaf => nil
-  | nil, _ => t :: nil
-  | Leaf :: q', _ => t :: q'
-  | u :: q', Leaf => u :: q'
-  | u :: q', _ => Leaf :: carry q' (smash t u)
-  end.
+  | nil, Leaf        => nil
+  | nil, _            => t :: nil
+  | Leaf :: q', _  => t :: q'
+  | u :: q', Leaf  => u :: q'
+  | u :: q', _       => Leaf :: carry q' (smash t u)
+ end.
 
-Definition insert (x : key) (q : priqueue) : priqueue :=
-  carry q (Node x Leaf Leaf).
+Definition insert (x: key) (q: priqueue) : priqueue :=
+     carry q (Node x Leaf Leaf).
 
-Fixpoint join (p q : priqueue) (c : tree) : priqueue :=
+Fixpoint join (p q: priqueue) (c: tree) : priqueue :=
   match p, q, c with
-  | [], _, _ => carry q c
-  | _, [], _ => carry p c
-  | Leaf :: p', Leaf :: q', _ => c :: join p' q' Leaf
-  | Leaf :: p', q1 :: q', Leaf => q1 :: join p' q' Leaf
-  | Leaf :: p', q1 :: q', Node _ _ _ =>
-      Leaf :: join p' q' (smash c q1)
-  | p1 :: p', Leaf :: q', Leaf => p1 :: join p' q' Leaf
-  | p1 :: p', Leaf :: q', Node _ _ _ =>
-      Leaf :: join p' q' (smash c p1)
-  | p1 :: p', q1 :: q', _ => c :: join p' q' (smash p1 q1)
+  | [], _ , _            => carry q c
+  | _, [], _             => carry p c
+  | Leaf::p', Leaf::q', _              => c :: join p' q' Leaf
+  | Leaf::p', q1::q', Leaf            => q1 :: join p' q' Leaf
+  | Leaf::p', q1::q', Node _ _ _  => Leaf :: join p' q' (smash c q1)
+  | p1::p', Leaf::q', Leaf            => p1 :: join p' q' Leaf
+  | p1::p', Leaf::q',Node _ _ _   => Leaf :: join p' q' (smash c p1)
+  | p1::p', q1::q', _                   => c :: join p' q' (smash p1 q1)
   end.
 
-(** First-order form of the original continuation-based [unzip]. *)
-Fixpoint unzip_acc (t : tree) (acc : priqueue) : priqueue :=
+Fixpoint unzip_acc (t: tree) (acc: priqueue) : priqueue :=
   match t with
-  | Leaf => acc
   | Node x t1 t2 => unzip_acc t2 (Node x t1 Leaf :: acc)
+  | Leaf => acc
   end.
 
-Definition unzip (t : tree) : priqueue :=
-  unzip_acc t [].
+Definition unzip (t: tree) : priqueue := unzip_acc t nil.
 
-Definition heap_delete_max (t : tree) : priqueue :=
+Definition heap_delete_max (t: tree) : priqueue :=
   match t with
-  | Node _ t1 Leaf => unzip t1
-  | _ => nil
+    Node x t1 Leaf  => unzip t1
+  | _ => nil   (* bogus value for ill-formed or empty trees *)
   end.
 
-Fixpoint find_max' (current : key) (q : priqueue) : key :=
+Fixpoint find_max' (current: key) (q: priqueue) : key :=
   match q with
-  | [] => current
-  | Leaf :: q' => find_max' current q'
-  | Node x _ _ :: q' =>
-      if x >? current then find_max' x q'
-      else find_max' current q'
+  |  []         => current
+  | Leaf::q' => find_max' current q'
+  | Node x _ _ :: q' => if x >? current then find_max' x q' else find_max' current q'
   end.
 
-Fixpoint find_max (q : priqueue) : option key :=
+Fixpoint find_max (q: priqueue) : option key :=
   match q with
   | [] => None
-  | Leaf :: q' => find_max q'
+  | Leaf::q' => find_max q'
   | Node x _ _ :: q' => Some (find_max' x q')
-  end.
+ end.
 
-Fixpoint delete_max_aux (m : key) (p : priqueue) : priqueue * priqueue :=
+Fixpoint delete_max_aux (m: key) (p: priqueue) : priqueue * priqueue :=
   match p with
-  | Leaf :: p' =>
-      let/d tmp := delete_max_aux m p' in
-      (Leaf :: fst tmp, snd tmp)
+  | Leaf :: p'   => dlet! tmp := delete_max_aux m p' in let (j,k) := tmp in (Leaf::j, k)
   | Node x t1 Leaf :: p' =>
-      if m >? x then
-        let/d tmp := delete_max_aux m p' in
-        (Node x t1 Leaf :: fst tmp, snd tmp)
-      else (Leaf :: p', heap_delete_max (Node x t1 Leaf))
-  | _ => (nil, nil)
+       if m >? x
+       then (dlet! tmp := delete_max_aux m p' in let (j,k) := tmp
+             in (Node x t1 Leaf::j,k))
+       else (Leaf::p', heap_delete_max (Node x t1 Leaf))
+  | _ => (nil, nil) (* Bogus value *)
   end.
 
-Definition delete_max (q : priqueue) : option (key * priqueue) :=
-  let/d mx := find_max q in
+Definition delete_max (q: priqueue) : option (key * priqueue) :=
+  dlet! mx := find_max q in
   match mx return option (key * priqueue) with
   | None => None
-  | Some m =>
-      let/d tmp := delete_max_aux m q in
-      Some (m, join (fst tmp) (snd tmp) Leaf)
+  | Some  m => dlet! tmp := delete_max_aux m q in let (p',q') := tmp
+                            in Some (m, join p' q' Leaf)
   end.
 
-Definition merge (p q : priqueue) : priqueue :=
-  join p q Leaf.
+Definition merge (p q: priqueue) := join p q Leaf.
 
-Fixpoint insert_list (l : list nat) (q : priqueue) : priqueue :=
-  match l with
-  | [] => q
-  | x :: l' => insert_list l' (insert x q)
-  end.
+Definition main_easy :=
+ let a := insert 5 (insert 3 (insert 7 empty)) in
+ let b := insert 3 (insert 6 (insert 9 empty)) in
+ let c := merge a b in
+ match delete_max c with
+ | Some (k, _) => k
+ | None => 0
+ end.
 
-Fixpoint make_list (n : nat) (l : list nat) : list nat :=
+Fixpoint insert_list (l : list nat) (q : priqueue) :=
+    match l with
+    | [] => q
+    | x :: l => insert_list l (insert x q)
+    end.
+
+Fixpoint make_list (n : nat) (l : list nat) :=
   match n with
   | 0 => 0 :: l
   | S 0 => 1 :: l
-  | S (S n') => make_list n' (S (S n') :: l)
+  | S (S n) => make_list n (S (S n) :: l)
   end.
 
-Definition benchmark_main : nat :=
-  let/d deleted := delete_max
-    (merge
-      (insert_list (make_list 2000 []) [])
-      (insert_list (make_list 2001 []) [])) in
+Definition benchmark_main :=
+  let a := insert_list (make_list 2000 []) nil in
+  let b := insert_list (make_list 2001 []) nil in
+  let c := merge a b in
+  dlet! deleted := delete_max c in
   match deleted return nat with
-  | Some answer => fst answer
+  | Some (k, _) => k
   | None => 0
   end.
-
-Lemma benchmark_main_result : benchmark_main = 2001.
-Proof. vm_compute. reflexivity. Qed.
